NCML/CK/Countermodel/TDia.lean
@@ -11,7 +11,7 @@ namespace CK
 
 open Model BDFormula
 
-namespace AscendingMRel
+namespace TDia
 
 def counterModel : Model (Fin 2) where
   iRel' x y := x = y
@@ -28,7 +28,7 @@ def counterModel : Model (Fin 2) where
 instance : counterModel.SerialMRel where
   serial_mRel _ := ⟨1, rfl⟩
 
-lemma counterModel_not_ascendingMRel : ¬ counterModel.AscendingMRel := by
+lemma counterModel_not_tDia : ¬ counterModel.TDia := by
   rintro ⟨h⟩;
   obtain ⟨z, Mz, hz⟩ := h 0;
   simp_all [counterModel, Frame.iRel, Frame.mRel, Frame.Fallible];
@@ -38,24 +38,24 @@ lemma counterModel_not_forces : 0 ⊮[counterModel] (#0 🡒 ◇(#0)) := by
   obtain ⟨z, Mz, hz⟩ := h 0 rfl rfl 0 rfl;
   simp_all [counterModel, Frame.mRel, Forces];
 
-end AscendingMRel
+end TDia
 
 instance : SerialMRel.counterModel.StrictlyAscendingMRel where
   strictly_ascending_mRel x := ⟨x, le_refl x, rfl⟩
 
-theorem exists_serialMRel_not_ascendingMRel :
-  ∃ (κ : Type) (M : Model κ), M.SerialMRel ∧ ¬M.AscendingMRel :=
-  ⟨Fin 2, AscendingMRel.counterModel, inferInstance, AscendingMRel.counterModel_not_ascendingMRel⟩
+theorem exists_serialMRel_not_tDia :
+  ∃ (κ : Type) (M : Model κ), M.SerialMRel ∧ ¬M.TDia :=
+  ⟨Fin 2, TDia.counterModel, inferInstance, TDia.counterModel_not_tDia⟩
 
-lemma exists_ascendingMRel_not_forces_N :
-  ∃ (κ : Type) (M : Model κ), M.AscendingMRel ∧ ∃ x : M.World, x ⊮[_] ∼◇⊥ :=
+lemma exists_tDia_not_forces_N :
+  ∃ (κ : Type) (M : Model κ), M.TDia ∧ ∃ x : M.World, x ⊮[_] ∼◇⊥ :=
   ⟨Fin 2, SerialMRel.counterModel, inferInstance, 0, SerialMRel.counterModel_not_forces⟩
 
 end CK
 
 lemma LogicCKD.not_provable_TDia : (#0 🡒 ◇(#0)) ∉ LogicCKD := by
   intro h;
-  apply CK.AscendingMRel.counterModel_not_forces (CK.Model.valid_of_mem_LogicCKD h 0)
+  apply CK.TDia.counterModel_not_forces (CK.Model.valid_of_mem_LogicCKD h 0)
 
 theorem LogicCKD.ssubset_CKTDia : LogicCKD ⊂ LogicCKTDia := by
   apply Set.ssubset_iff_exists.mpr;
